WIP: Use Std.Hashmap Lemmas

CertifyingDatalog/GraphValidation/Basic.lean
@@ -1,20 +1,107 @@
 import CertifyingDatalog.Basic
 import CertifyingDatalog.Datalog
 
-abbrev PreGraph (A: Type u) [DecidableEq A] [Hashable A] := Batteries.HashMap A (List A)
+theorem Std.HashMap.mem_keys_iff_contains [DecidableEq A] [Hashable A] (hm : Std.HashMap A B) (k : A) : k ∈ hm.keys ↔ hm.contains k := by
+  unfold keys
+  unfold Std.DHashMap.keys
+  unfold Std.DHashMap.Raw.keys
+  unfold Std.DHashMap.Raw.fold
+  unfold Std.DHashMap.Raw.foldM
+  rw [Array.foldlM_eq_foldlM_data, List.foldlM_eq_foldl]
+
+  unfold contains
+  unfold Std.DHashMap.contains
+  unfold Std.DHashMap.Internal.Raw₀.contains
+
+  simp
+  sorry
+
+theorem Std.HashMap.ofList_mapped_to_pair_contains_iff_list_elem [DecidableEq A] [Hashable A] (l : List A) (a : A) : ∀ b : B, (Std.HashMap.ofList (l.map (fun a => (a, b)))).contains a ↔ a ∈ l := by
+  intro b
+  unfold ofList
+  unfold DHashMap.Const.ofList
+  unfold DHashMap.Const.insertMany
+  unfold contains
+  simp
+
+  have : ∀ hm : HashMap A B, (List.foldl (fun m x => m.insert x.1 x.2) hm (List.map (fun a => (a, b)) l)).contains a = true ↔ hm.contains a ∨ a ∈ l := by
+    induction l with
+    | nil => simp
+    | cons head tail ih =>
+      simp
+      intro hm
+      rw [ih (hm.insert head b)]
+      rw [contains_insert]
+      simp
+      have : a = head ↔ head = a := by constructor <;> apply Eq.symm
+      rw [this]
+      conv => left; left; rw [or_comm]
+      rw [or_assoc]
+
+  have applied_this := this empty
+  simp at applied_this
+  sorry
+  /- apply applied_this -/
+
+theorem Std.HashMap.getD_ofList_is_list_find_getD [DecidableEq A] [Hashable A] (l : List (A × B)) (a : A) : ∀ b, (Std.HashMap.ofList l).getD a b = ((l.reverse.find? (fun x => x.fst == a)).map Prod.snd).getD b := by
+  intro b
+  unfold ofList
+  /- simp -/
+
+  have : ∀ hm : HashMap A B, (List.foldl (fun m x => m.insert x.1 x.2) hm l).getD a b = (Option.map Prod.snd (List.find? (fun x => x.1 == a) l.reverse)).getD (hm.getD a b) := by
+    induction l with
+    | nil => simp
+    | cons head tail ih =>
+      simp
+      intro hm
+      rw [ih (hm.insert head.1 head.2)]
+      rw [getD_insert]
+      split
+      case isTrue h =>
+        have : (tail.reverse ++ [head]).find? (fun x => x.1 == a) = (tail.reverse.find? (fun x => x.1 == a)).getD head := by
+          rw [List.find_concat]
+          have : [head].find? (fun x => x.1 == a) = some head := by unfold List.find?; simp [h]
+          rw [this]
+          have : ∀ {α} (opt : Option α) (x : α), opt.orElse (fun _ => some x) = Option.some (opt.getD x) := by
+            intro _ opt x
+            unfold Option.orElse
+            split <;> simp
+          rw [this]
+        rw [this]
+        simp
+      case isFalse h =>
+        have : (tail.reverse ++ [head]).find? (fun x => x.1 == a) = tail.reverse.find? (fun x => x.1 == a) := by
+          rw [List.find_concat]
+          have : (head.1 == a) = false := by simp; simp at h; exact h
+          have : [head].find? (fun x => x.1 == a) = none := by unfold List.find?; simp [this]
+          rw [this]
+          have : ∀ {α} (opt : Option α), opt.orElse (fun _ => none) = opt := by
+            intro _ opt
+            unfold Option.orElse
+            split <;> simp
+          rw [this]
+        rw [this]
+
+  sorry
+  /- rw [this] -/
+  /- rw [findD_is_default_when_not_contains] -/
+  /- simp -/
+  /- apply empty_contains -/
+
+abbrev PreGraph (A: Type u) [DecidableEq A] [Hashable A] := Std.HashMap A (List A)
 
 namespace PreGraph
   variable {A: Type u} [DecidableEq A] [Hashable A]
 
-  def vertices (g : PreGraph A) : List A := g.toList.map Prod.fst
-  def predecessors (g : PreGraph A) (a : A) : List A := g.findD a []
+  def vertices (g : PreGraph A) : List A := g.keys
+  def predecessors (g : PreGraph A) (a : A) : List A := g.getD a []
 
   def complete (pg: PreGraph A) := ∀ (a:A), pg.contains a →  ∀ (a':A), a' ∈ (pg.predecessors a) → pg.contains a'
 
-  theorem in_vertices_iff_contains (pg: PreGraph A) (a : A) : a ∈ pg.vertices ↔ pg.contains a := by unfold vertices; apply Batteries.HashMap.in_projection_of_toList_iff_contains
-  theorem in_predecessors_iff_found (pg: PreGraph A) (a : A) : ∀ b, b ∈ pg.predecessors a ↔ b ∈ (pg.findD a []) := by unfold predecessors; intros; rfl
+  theorem in_vertices_iff_contains (pg: PreGraph A) (a : A) : a ∈ pg.vertices ↔ pg.contains a := by unfold vertices; apply Std.HashMap.mem_keys_iff_contains
+  theorem in_predecessors_iff_found (pg: PreGraph A) (a : A) : ∀ b, b ∈ pg.predecessors a ↔ b ∈ (pg.getD a []) := by unfold predecessors; intros; rfl
 
-  def from_vertices (vs : List A) : PreGraph A := Batteries.HashMap.ofList (vs.map (fun v => (v, [])))
+  def from_vertices (vs : List A) : PreGraph A := Std.HashMap.ofList (vs.map (fun v => (v, [])))
 
   def add_vertex (pg : PreGraph A) (v : A) : PreGraph A :=
     if pg.contains v then
@@ -41,13 +128,14 @@ namespace PreGraph
         split at hl
         apply Or.inl
         exact hl
-        rw [Batteries.HashMap.contains_insert] at hl
+        rw [Std.HashMap.contains_insert] at hl
         cases Decidable.em (pg.contains v) with
         | inl v_in_pg => apply Or.inl; exact v_in_pg
         | inr v_not_in_pg =>
+          simp at hl
           cases hl with
-          | inl _ => contradiction
-          | inr hl => apply Or.inr; constructor; simp at v_not_in_pg; exact v_not_in_pg; apply Or.inl; apply Eq.symm; exact LawfulBEq.eq_of_beq hl
+          | inl hl => apply Or.inr; constructor; simp at v_not_in_pg; exact v_not_in_pg; apply Or.inl; apply Eq.symm; exact hl
+          | inr _ => contradiction
       | inr hr =>
         unfold add_vertex at hr
         split at hr
@@ -57,7 +145,7 @@ namespace PreGraph
         exact hr.left
         apply Or.inr
         exact hr.right
-        rw [Batteries.HashMap.contains_insert] at hr
+        rw [Std.HashMap.contains_insert] at hr
         cases Decidable.em (pg.contains v) with
         | inl v_in_pg => apply Or.inl; exact v_in_pg
         | inr v_not_in_pg => apply Or.inr; constructor; simp at v_not_in_pg; exact v_not_in_pg; apply Or.inr; exact hr.right
@@ -68,8 +156,9 @@ namespace PreGraph
         unfold add_vertex
         split
         exact hl
-        rw [Batteries.HashMap.contains_insert]
-        apply Or.inl
+        rw [Std.HashMap.contains_insert]
+        simp
+        apply Or.inr
         exact hl
       | inr hr =>
         let ⟨hrl, hrr⟩ := hr
@@ -82,10 +171,10 @@ namespace PreGraph
             apply False.elim; rw [v_is_u] at hrl
             have : ¬ pg.contains u := by simp [hrl]
             contradiction
-          rw [Batteries.HashMap.contains_insert]
-          apply Or.inr
-          rw [v_is_u]
+          rw [Std.HashMap.contains_insert]
           simp
+          apply Or.inl
+          rw [v_is_u]
         | inr v_in_us =>
           cases Decidable.em ((pg.add_vertex u).contains v)
           apply Or.inl
@@ -95,7 +184,7 @@ namespace PreGraph
           assumption
           exact v_in_us
 
-  theorem add_vertices_findD_semantics (pg : PreGraph A) (vs : List A) (a : A): (pg.add_vertices vs).findD a [] = pg.findD a [] := by
+  theorem add_vertices_getD_semantics (pg : PreGraph A) (vs : List A) (a : A): (pg.add_vertices vs).getD a [] = pg.getD a [] := by
     induction vs generalizing pg with
     | nil => simp [add_vertices]
     | cons u us ih =>
@@ -105,9 +194,16 @@ namespace PreGraph
       rw [ih_plugged_in]
       unfold add_vertex
       split
-      rfl
-      rw [Batteries.HashMap.findD_insert]
-      assumption
+      . rfl
+      case isFalse h =>
+        rw [Std.HashMap.getD_insert]
+        simp
+        intro eq
+        apply Eq.symm
+        apply Std.HashMap.getD_eq_fallback_of_contains_eq_false
+        rw [← eq]
+        simp at h
+        exact h
 
   def add_vertex_with_predecessors (pg : PreGraph A) (v : A) (vs : List A) : PreGraph A :=
     let pg_with_added_predecessors := if pg.contains v then pg.insert v ((pg.predecessors v) ++ vs) else pg.insert v vs
@@ -117,16 +213,16 @@ namespace PreGraph
     unfold vertices
     unfold from_vertices
     intro v
-    rw [Batteries.HashMap.in_projection_of_toList_iff_contains, Batteries.HashMap.ofList_mapped_to_pair_contains_iff_list_elem]
+    rw [Std.HashMap.mem_keys_iff_contains, Std.HashMap.ofList_mapped_to_pair_contains_iff_list_elem]
 
-  theorem from_vertices_no_vertex_has_predecessors (vs : List A) : ∀ v, (PreGraph.from_vertices vs).findD v [] = [] := by
+  theorem from_vertices_no_vertex_has_predecessors (vs : List A) : ∀ v, (PreGraph.from_vertices vs).getD v [] = [] := by
     intro needle
     unfold from_vertices
-    rw [Batteries.HashMap.findD_ofList_is_list_find_getD]
+    rw [Std.HashMap.getD_ofList_is_list_find_getD]
 
-    induction vs with 
+    induction vs with
     | nil => simp
-    | cons v vs ih => 
+    | cons v vs ih =>
       simp
       rw [List.find_concat]
 
@@ -140,7 +236,7 @@ namespace PreGraph
 
   theorem from_vertices_is_complete (vs : List A) : (PreGraph.from_vertices vs).complete := by
     let pg := PreGraph.from_vertices vs
-    have : ∀ v, pg.findD v [] = [] := by
+    have : ∀ v, pg.getD v [] = [] := by
       intro v
       apply from_vertices_no_vertex_has_predecessors
     intro a ha b hb
@@ -160,55 +256,53 @@ namespace PreGraph
     | inl hl =>
       split at hl
       case isTrue hl' =>
-        rw [Batteries.HashMap.contains_insert] at hl
+        rw [Std.HashMap.contains_insert] at hl
+        simp at hl
         cases hl with
         | inl hll =>
-          cases Decidable.em (a = v) with
-          | inl a_eq_v => apply Or.inl; constructor; exact hll; exact a_eq_v
-          | inr a_neq_v => apply Or.inr; apply Or.inl; constructor; exact hll; exact a_neq_v
-        | inr hlr =>
-          have : v = a := by apply LawfulBEq.eq_of_beq; apply hlr
           apply Or.inl
           constructor
-          rw [← this]
+          rw [← hll]
           apply hl'
-          rw [this]
+          rw [hll]
+        | inr hlr =>
+          cases Decidable.em (a = v) with
+          | inl a_eq_v => apply Or.inl; constructor; exact hlr; exact a_eq_v
+          | inr a_neq_v => apply Or.inr; apply Or.inl; constructor; exact hlr; exact a_neq_v
       case isFalse hr' =>
-        rw [Batteries.HashMap.contains_insert] at hl
+        rw [Std.HashMap.contains_insert] at hl
+        simp at hl
         cases hl with
         | inl hll =>
-          cases Decidable.em (a = v) with
-          | inl a_eq_v => apply Or.inl; constructor; exact hll; exact a_eq_v
-          | inr a_neq_v => apply Or.inr; apply Or.inl; constructor; exact hll; exact a_neq_v
-        | inr hlr =>
-          have : v = a := by apply LawfulBEq.eq_of_beq; apply hlr
           apply Or.inr
           apply Or.inr
           apply Or.inl
           constructor
-          rw [← this]
+          rw [← hll]
           simp at hr'
           apply hr'
-          rw [this]
+          rw [hll]
+        | inr hlr =>
+          cases Decidable.em (a = v) with
+          | inl a_eq_v => apply Or.inl; constructor; exact hlr; exact a_eq_v
+          | inr a_neq_v => apply Or.inr; apply Or.inl; constructor; exact hlr; exact a_neq_v
     | inr hr =>
       let ⟨hrl, hrr⟩ := hr
       split at hrl
       case isTrue hl' =>
-        rw [Batteries.HashMap.contains_insert] at hrl
+        rw [Std.HashMap.contains_insert] at hrl
+        simp at hrl
         cases Decidable.em (a = v) with
         | inl a_eq_v =>
-          apply False.elim
-          apply hrl
-          apply Or.inr
-          rw [a_eq_v]
-          simp
+          rw [a_eq_v] at hrl
+          have contra := hrl.left
+          contradiction
         | inr a_neq_v =>
           cases Decidable.em (pg.contains a) with
           | inl pg_contains =>
-            apply False.elim
-            apply hrl
-            apply Or.inl
-            rw [pg_contains]
+            rw [pg_contains] at hrl
+            have contra := hrl.right
+            contradiction
           | inr pg_not_contains =>
             apply Or.inr
             apply Or.inr
@@ -220,21 +314,19 @@ namespace PreGraph
             apply a_neq_v
             apply hrr
       case isFalse hr' =>
-        rw [Batteries.HashMap.contains_insert] at hrl
+        rw [Std.HashMap.contains_insert] at hrl
+        simp at hrl
         cases Decidable.em (a = v) with
         | inl a_eq_v =>
-          apply False.elim
-          apply hrl
-          apply Or.inr
-          rw [a_eq_v]
-          simp
+          rw [a_eq_v] at hrl
+          have contra := hrl.left
+          contradiction
         | inr a_neq_v =>
           cases Decidable.em (pg.contains a) with
           | inl pg_contains =>
-            apply False.elim
-            apply hrl
-            apply Or.inl
-            rw [pg_contains]
+            rw [pg_contains] at hrl
+            have contra := hrl.right
+            contradiction
           | inr pg_not_contains =>
             apply Or.inr
             apply Or.inr
@@ -251,115 +343,110 @@ namespace PreGraph
     | inl hll =>
       apply Or.inl
       split
-      rw [Batteries.HashMap.contains_insert]
+      rw [Std.HashMap.contains_insert]
+      simp
       apply Or.inl
-      exact hll.left
-      rw [Batteries.HashMap.contains_insert]
+      rw [hll.right]
+      rw [Std.HashMap.contains_insert]
+      simp
       apply Or.inl
-      exact hll.left
+      rw [hll.right]
     | inr hlr => cases hlr with
     | inl hll =>
       apply Or.inl
       split
-      rw [Batteries.HashMap.contains_insert]
-      apply Or.inl
-      exact hll.left
-      rw [Batteries.HashMap.contains_insert]
-      apply Or.inl
-      exact hll.left
+      rw [Std.HashMap.contains_insert]
+      simp
+      apply Or.inr
+      rw [hll.left]
+      rw [Std.HashMap.contains_insert]
+      simp
+      apply Or.inr
+      rw [hll.left]
     | inr hlr => cases hlr with
     | inl hll =>
       apply Or.inl
       split
-      rw [Batteries.HashMap.contains_insert]
+      rw [Std.HashMap.contains_insert]
+      simp
       apply Or.inr
       rw [hll.right]
+      assumption
+      rw [Std.HashMap.contains_insert]
       simp
-      rw [Batteries.HashMap.contains_insert]
-      apply Or.inr
+      apply Or.inl
       rw [hll.right]
-      simp
     | inr hlr =>
       apply Or.inr
       split
-      rw [Batteries.HashMap.contains_insert]
+      rw [Std.HashMap.contains_insert]
+      simp
+      constructor
       constructor
       intro contra
-      cases contra
-      have : ¬ pg.contains a := by simp [hlr.left]
-      contradiction
-      case inr v_is_a =>
-        have : a = v := by apply Eq.symm; exact LawfulBEq.eq_of_beq v_is_a
-        have : a ≠ v := hlr.right.left
-        contradiction
-      exact hlr.right.right
-      rw [Batteries.HashMap.contains_insert]
+      apply hlr.right.left
+      rw [contra]
+      apply hlr.left
+      apply hlr.right.right
       constructor
       intro contra
-      cases contra
-      have : ¬ pg.contains a := by simp [hlr.left]
-      contradiction
-      case inr v_is_a =>
-        have : a = v := by apply Eq.symm; exact LawfulBEq.eq_of_beq v_is_a
-        have : a ≠ v := hlr.right.left
-        contradiction
-      exact hlr.right.right
+      rw [Std.HashMap.contains_insert] at contra
+      simp at contra
+      cases contra with
+      | inl contra => apply hlr.right.left; rw [contra]
+      | inr contra => have contra' := hlr.left; rw [contra'] at contra; contradiction
+      apply hlr.right.right
 
-  theorem add_vertex_with_predecessors_findD_semantics_1 (pg : PreGraph A) (v a : A) (vs : List A) (h : pg.contains a ∧ a = v) : (pg.add_vertex_with_predecessors v vs).findD a [] = (pg.predecessors v) ++ vs := by
+  theorem add_vertex_with_predecessors_getD_semantics_1 (pg : PreGraph A) (v a : A) (vs : List A) (h : pg.contains a ∧ a = v) : (pg.add_vertex_with_predecessors v vs).getD a [] = (pg.predecessors v) ++ vs := by
     unfold add_vertex_with_predecessors
     simp
-    rw [add_vertices_findD_semantics]
+    rw [add_vertices_getD_semantics]
     rw [← h.right]
     simp [h.left]
-    rw [Batteries.HashMap.findD_insert']
 
-  theorem add_vertex_with_predecessors_findD_semantics_2 (pg : PreGraph A) (v a : A) (vs : List A) (h : pg.contains a ∧ a ≠ v) : (pg.add_vertex_with_predecessors v vs).findD a [] = (pg.predecessors a) := by
+  theorem add_vertex_with_predecessors_getD_semantics_2 (pg : PreGraph A) (v a : A) (vs : List A) (h : pg.contains a ∧ a ≠ v) : (pg.add_vertex_with_predecessors v vs).getD a [] = (pg.predecessors a) := by
     unfold add_vertex_with_predecessors
     simp
-    rw [add_vertices_findD_semantics]
+    rw [add_vertices_getD_semantics]
     split
-    rw [Batteries.HashMap.findD_insert'']
+    rw [Std.HashMap.getD_insert]
+    simp
+    split
+    case isTrue eq => have h_right := h.right; rw [eq] at h_right; contradiction
     unfold predecessors
     rfl
-    have contra := h.right
-    intro contra'
-    rw [contra'] at contra
-    contradiction
-    rw [Batteries.HashMap.findD_insert'']
+    rw [Std.HashMap.getD_insert]
+    simp
+    split
+    case isTrue eq => have h_right := h.right; rw [eq] at h_right; contradiction
     unfold predecessors
     rfl
-    have contra := h.right
-    intro contra'
-    rw [contra'] at contra
-    contradiction
 
-  theorem add_vertex_with_predecessors_findD_semantics_3 (pg : PreGraph A) (v a : A) (vs : List A) (h : (¬ pg.contains a) ∧ a = v) : (pg.add_vertex_with_predecessors v vs).findD a [] = vs := by
+  theorem add_vertex_with_predecessors_getD_semantics_3 (pg : PreGraph A) (v a : A) (vs : List A) (h : (¬ pg.contains a) ∧ a = v) : (pg.add_vertex_with_predecessors v vs).getD a [] = vs := by
     unfold add_vertex_with_predecessors
     simp
-    rw [add_vertices_findD_semantics]
+    rw [add_vertices_getD_semantics]
     rw [← h.right]
     simp [h.left]
-    rw [Batteries.HashMap.findD_insert']
 
-  theorem add_vertex_with_predecessors_findD_semantics_4 (pg : PreGraph A) (v a : A) (vs : List A) (h : (¬ pg.contains a) ∧ a ≠ v) : (pg.add_vertex_with_predecessors v vs).findD a [] = [] := by
+  theorem add_vertex_with_predecessors_getD_semantics_4 (pg : PreGraph A) (v a : A) (vs : List A) (h : (¬ pg.contains a) ∧ a ≠ v) : (pg.add_vertex_with_predecessors v vs).getD a [] = [] := by
     unfold add_vertex_with_predecessors
     simp
-    rw [add_vertices_findD_semantics]
+    simp at h
+    rw [add_vertices_getD_semantics]
     split
-    rw [Batteries.HashMap.findD_insert'']
-    rw [Batteries.HashMap.findD_is_default_when_not_contains]
-    exact h.left
-    have contra := h.right
-    intro contra'
-    rw [contra'] at contra
-    contradiction
-    rw [Batteries.HashMap.findD_insert'']
-    rw [Batteries.HashMap.findD_is_default_when_not_contains]
-    exact h.left
-    have contra := h.right
-    intro contra'
-    rw [contra'] at contra
-    contradiction
+    rw [Std.HashMap.getD_insert]
+    simp
+    split
+    case isTrue eq => have h_right := h.right; rw [eq] at h_right; contradiction
+    rw [Std.HashMap.getD_eq_fallback_of_contains_eq_false]
+    apply h.left
+    rw [Std.HashMap.getD_insert]
+    simp
+    split
+    case isTrue eq => have h_right := h.right; rw [eq] at h_right; contradiction
+    rw [Std.HashMap.getD_eq_fallback_of_contains_eq_false]
+    apply h.left
 
   theorem add_vertex_with_predecessors_still_complete (pg : PreGraph A) (v : A) (vs : List A) (pg_is_complete : pg.complete) : (pg.add_vertex_with_predecessors v vs).complete := by
     unfold complete
@@ -370,7 +457,7 @@ namespace PreGraph
     rw [add_vertex_with_predecessors_contains_iff_contains_or_in_new_vertices]
     cases ha with
     | inl contains_and_eq =>
-      rw [add_vertex_with_predecessors_findD_semantics_1 pg v a _ contains_and_eq] at ha'
+      rw [add_vertex_with_predecessors_getD_semantics_1 pg v a _ contains_and_eq] at ha'
       rw [List.mem_append_eq] at ha'
       cases ha' with
       | inl ha' =>
@@ -389,13 +476,13 @@ namespace PreGraph
           | inr hrr => apply Or.inr; apply Or.inr; apply Or.inr; constructor; exact hrr; constructor; exact hr; exact ha'
     | inr rest => cases rest with
     | inl contains_and_neq =>
-      rw [add_vertex_with_predecessors_findD_semantics_2 pg v a _ contains_and_neq] at ha'
+      rw [add_vertex_with_predecessors_getD_semantics_2 pg v a _ contains_and_neq] at ha'
       cases Decidable.em (a' = v) with
       | inl hl => apply Or.inl; constructor; apply pg_is_complete; exact contains_and_neq.left; apply ha'; exact hl
       | inr hr => apply Or.inr; apply Or.inl; constructor; apply pg_is_complete; exact contains_and_neq.left; apply ha'; exact hr
     | inr rest => cases rest with
     | inl not_contains_and_eq =>
-      rw [add_vertex_with_predecessors_findD_semantics_3 pg v a _ not_contains_and_eq] at ha'
+      rw [add_vertex_with_predecessors_getD_semantics_3 pg v a _ not_contains_and_eq] at ha'
       cases Decidable.em (a' = v) with
       | inl hl =>
         cases Decidable.em (pg.contains a') with
@@ -406,14 +493,14 @@ namespace PreGraph
         | inl hrl => apply Or.inr; apply Or.inl; constructor; exact hrl; exact hr
         | inr hrr => apply Or.inr; apply Or.inr; apply Or.inr; constructor; exact hrr; constructor; exact hr; exact ha'
     | inr not_contains_and_neq =>
-      rw [add_vertex_with_predecessors_findD_semantics_4 pg v a _ (⟨not_contains_and_neq.left, not_contains_and_neq.right.left⟩)] at ha'
+      rw [add_vertex_with_predecessors_getD_semantics_4 pg v a _ (⟨not_contains_and_neq.left, not_contains_and_neq.right.left⟩)] at ha'
       contradiction
 end PreGraph
 
 abbrev Graph (A: Type u) [DecidableEq A] [Hashable A] := { pg : PreGraph A // pg.complete }
 
 namespace Graph
-  variable {A: Type u} [DecidableEq A] [Hashable A] 
+  variable {A: Type u} [DecidableEq A] [Hashable A]
 
   def vertices (g : Graph A) : List A := g.val.vertices
   def predecessors (g : Graph A) (a : A) : List A := g.val.predecessors a
@@ -440,27 +527,30 @@ namespace Graph
       property := by apply PreGraph.add_vertex_with_predecessors_still_complete; apply g.property
     }
 
-  theorem mem_of_has_pred (G : Graph A) (a b : A) : b ∈ G.predecessors a -> a ∈ G.vertices := by 
+  theorem mem_of_has_pred (G : Graph A) (a b : A) : b ∈ G.predecessors a -> a ∈ G.vertices := by
     intro b_pred
     unfold predecessors at b_pred
     rw [PreGraph.in_predecessors_iff_found] at b_pred
-    rw [Batteries.HashMap.findD_eq_find?] at b_pred
-    cases eq : Batteries.HashMap.find? G.val a with
-    | none => simp [eq] at b_pred
-    | some _ =>
+    cases eq : G.val.contains a with
+    | false =>
+      rw [Std.HashMap.getD_eq_fallback_of_contains_eq_false] at b_pred
+      contradiction
+      exact eq
+    | true =>
       unfold vertices
       rw [PreGraph.in_vertices_iff_contains]
-      apply Batteries.HashMap.contains_of_find?
       exact eq
 
-  theorem mem_of_is_pred (G : Graph A) (a b : A) : b ∈ G.predecessors a -> b ∈ G.vertices := by 
+  theorem mem_of_is_pred (G : Graph A) (a b : A) : b ∈ G.predecessors a -> b ∈ G.vertices := by
     intro b_pred
     unfold predecessors at b_pred
     rw [PreGraph.in_predecessors_iff_found] at b_pred
-    rw [Batteries.HashMap.findD_eq_find?] at b_pred
-    cases eq : Batteries.HashMap.find? G.val a with
-    | none => simp [eq] at b_pred
-    | some _ =>
+    cases eq : G.val.contains a with
+    | false =>
+      rw [Std.HashMap.getD_eq_fallback_of_contains_eq_false] at b_pred
+      contradiction
+      exact eq
+    | true =>
       apply complete
       apply mem_of_has_pred
       apply b_pred
